\documentclass[10pt]{article}
 
\usepackage[margin=1in]{geometry} 
\usepackage{amsmath,amsthm,amssymb, graphicx, multicol, array, enumerate, gensymb}
\newcommand{\N}{\mathbb{N}}
\newcommand{\Z}{\mathbb{Z}}
 
\newenvironment{problem}[2][Problem]{\begin{trivlist}
\item[\hskip \labelsep {\bfseries #1}\hskip \labelsep {\bfseries #2.}]}{\end{trivlist}}

\begin{document}
 
\title{Mathematics solutions}
\date{}
\maketitle

 \section{Elementary algebra}
 
\begin{problem}{1.1}
 $$\frac{x^{n+2}}{x^{n-2}}=x^{n+2-n-2}=x^4$$
\end{problem}

\begin{problem}{1.2}
$$x^{-1}*8=2$$ $${x}\neq{0}$$
$$\frac{8}{x}=2$$ 
$${x}=\frac{8}{2}=4$$

\end{problem}

\begin{problem}{1.3}
$$(a^b)^0=(5^10)^0=5^0=1$$
\end{problem}

\begin{problem}{1.4}
$$\frac{\sqrt{4x}}{\sqrt{x}}=2\frac{\sqrt{x}}{\sqrt{x}}=2$$
\end{problem}

\begin{problem}{1.5}
$$x^2+(x+1)^2=(x+2)^2$$
$$x^2+(x^2+2x+1)=x^2+4x+4$$
$$x^2-2x-3=0$$
$$D=4+4*3=16$$
$$x=\frac{2-4}{2}=-1$$
$$x=\frac{2+4}{2}=3$$
\end{problem}

\begin{problem}{1.6}
$$2^x>1024$$
$$2^x>2^10$$
$$x>10$$
\end{problem}

\section{Functions of one variable}

\begin{problem}{2.1 (Based on SYD 2.5.6)}
$$y=kx+b$$
where x is the temperature in Celsius and y is temperature in Fahrenheit 
$$32=k*0+b$$
$$212=k*100+b$$
$$b=32$$
$$212=100k+32$$
$$100k=180$$
$$k=1.8$$
$$x=y$$
$$x=32+1.8x$$
$$-0.8x=32$$
$$x=y=-40$$
\end{problem}

\begin{problem}{2.2}
$f(3)=5x+4=5*3+4=15+4=19$
\end{problem}

\begin{problem}{2.3}
$$x^2-4x+3=0$$
$$D=4^2-4*3=16-12=4$$
$$x=\frac{4-2}{2}=1$$
$$x=\frac{4+2}{2}=3$$

\end{problem}

\begin{problem}{2.4}
$$10*(1+0.02)^90)=60858$$
\end{problem}

\begin{problem}{2.5}

$$e^{\ln 5}=5$$
\end{problem}

\section{Calculus}

\begin{problem}{3.1}
$$\sum\limits_{i=1}^{\infty} \frac{12}{6^i}=\frac{12*\frac{1}{6}}{1-\frac{1}{6}}=\frac{2}{\frac{5}{6}}=\frac{2*6}{5}=2.4$$
\end{problem}

\begin{problem}{3.2}
$$\lim\limits_{x \rightarrow 1}\frac{6^{1-x}}{x}=\lim\limits_{x \rightarrow 1}\frac{6^{1-x}*6^x}{x*6^x}=\lim\limits_{x \rightarrow 1}\frac{6}{1*6}=1$$
\end{problem}

\begin{problem}{3.3}
$f(x)=x^5-8$
$$f'(x)=5x^4$$
$$f'(3)=5*3^4=405$$
\end{problem}

\begin{problem}{3.4}
$$\frac{\mathrm{d}}{\mathrm{d}\, x} \frac{x^3+2x-1}{x-2}$$
$$\frac{\mathrm{d}}{\mathrm{d}\, x} \frac{(3x^3+2x)(x-2)-(x^3+2x-1)}{(x-2)^2}=\frac{3x^3-6x^2+2x-4-x^3-2x+1}{(x-2)^2}=\frac{2x^3-6x^2-3}{(x-2)^2}$$
\end{problem}

\begin{problem}{3.5}
$$\frac{\mathrm{d}}{\mathrm{d}\, x} 4x^4+4x^2=16x^3+8x$$
 $$\frac{\mathrm{d^2}}{\mathrm{d}\, x^2} 4x^4+4x^2=\frac{\mathrm{d}}{\mathrm{d}\, x} 16x^3+8x=48x^2+8 $$

 
\end{problem}

\begin{problem}{3.6}

$$\frac{\mathrm{d}}{\mathrm{d}\, x} \frac{\ln x}{e^x}=\frac{\mathrm{d}}{\mathrm{d}\, x} \frac{\frac{e^x}{x}-\frac{e^x}{\ln x}}{e^{2x}}=\frac{\frac{e^x}{x}-\frac{e^x}{\ln{x}}}{e^{2x}}=\frac{1}{xe^x}-\frac{1}{x\ln{x}}$$
\end{problem}

\begin{problem}{3.7}

$$f(x)=3x^2-5x+2$$
$$f'(x)=6x-5=$$
$$6x=5$$
$$x=\frac{5}{6}$$

\begin{center}
 \begin{tabular}{||c c c c||} 
 \hline
 x & $<\frac{5}{6}$ & $\frac{5}{6}$ & $>\frac{5}{6}$ \\ [0.5ex] 
 \hline\hline
 $f'{x}$ & - & 0 & + \\
 \hline
 Slope & decreasing & min & increasing \\
 \hline
 $f''{x}$ & + & + & + \\
 \hline
 Convexity & convex & convex & convex \\ [1ex] 
 \hline
\end{tabular}
\end{center}
\end{problem}

\begin{problem}{3.8}
$f(x,y)=x^2+y^3$ 
$$f(2,3)=2^2+3^3=4+9=13$$
\end{problem}

\begin{problem}{3.9}
$f(x,y)=\ln(x-y)$
$$x-y>0$$
$$x>y$$
\end{problem}

\begin{problem}{3.10}
$$\frac{\partial}{\partial \, x} x^5+xy^3=5x^4+y^3$$
\end{problem}

\begin{problem}{3.11}
$$f(x,y)=x^2y^2+10$$
$$\frac{\partial}{\partial \, x} x^2y^2+10=2xy^2$$
$$\frac{\partial}{\partial \, y} x^2y^2+10=2yx^2$$
$$2xy^2=2yx^2=0$$
$$y=x=0$$
As the function is convex, the stationary point (0,0) is a local minima.
\end{problem}

\begin{problem}{3.12}

$\max x^2y^2$ s.t. $x+y=10$
$$\frac{\partial}{\partial \, x} x^2y^2=2xy^2$$
$$\frac{\partial}{\partial \, y} x^2y^2=2yx^2$$
$$2xy^2=2yx^2$$
$$x=y$$
$$2x=10$$
$$x=y=5$$
\end{problem}

\section{Linear algebra}

\begin{problem}{4.1}

$$A=\begin{bmatrix} 2 & 6\\ 5 & 1 \\ 1 & 9\end{bmatrix}$$
$$B=\begin{bmatrix} 1 & 1 & 7\\2 & 8 & 2\end{bmatrix}$$

  $$A \cdot B=\begin{bmatrix} 2 & 2\\ 4 & 6 \\ 1 & 3\end{bmatrix}\cdot \begin{bmatrix} 1 & 1 & 7\\2 & 8 & 2\end{bmatrix}=\begin{bmatrix} 14 & 50 & 26\\7 & 13 & 37\\ 19 & 73 & 25 \end{bmatrix}$$
 
\end{problem}

\begin{problem}{4.2}
Take the following matrices:
$$A=\begin{bmatrix} 2 & 2\\ 4 & 6 \\ 1 & 3\end{bmatrix}$$
$$B=\begin{bmatrix} 1 & 9 & 1\\2 & 1 & 2\end{bmatrix}$$
$$A \cdot B=\begin{bmatrix} 2 & 2\\ 4 & 6 \\ 1 & 3\end{bmatrix}\cdot \begin{bmatrix} 1 & 9 & 1\\2 & 1 & 2\end{bmatrix}=\begin{bmatrix} 39 & 59\\ 10 & 16 \end{bmatrix}$$
\end{problem}

\begin{problem}{4.3}

$$\begin{bmatrix}7.1 & 9.1 & 4.7\\ 2 & 7.8 & 1.1 \\ 4 & 4.44 & 0\end{bmatrix}^T=\begin{bmatrix}7.1 & 2 & 4\\ 9.1 & 7.8 & 4.44 \\ 4.7 & 1.1 & 0\end{bmatrix}$$
\end{problem}

\begin{problem}{4.4}

$$\begin{bmatrix}1 & 9 \\ 2 & 8 \end{bmatrix} $$
$D=1*8-2*9=8-18=-10$
\end{problem}

\section{Probability theory}

\begin{problem}{5.1}
\begin{tabular}{llllll}
 11 & 12 & 13  & 14 & 15 & 16 \\
 21 & 22 & 23  & 24 & 25 & 26 \\
 31 & 32 & 33  & 34 & 35 & 36 \\
 41 & 42 & 43  & 44 & 45 & 46 \\
 51 & 52 & 53  & 54 & 55 & 56 \\
 61 & 62 & 63  & 64 & 65 & 66 \ 
\end{tabular}
\end{problem}

\begin{problem}{5.2+5.3}
$$
$$\begin{tabular}{llll} 
\hline
 & Uses Drugs (D) & Doesn't Use Drugs (D') & Total \\ 
\hline
Positive Test Results (T) & P(T\cap D) & P(T\cap D') & P(T) \\ 
\hline
Negative Test Results (T') & P(T'\cap D) & P(T'\cap D') & P(T') \\ 
\hline
\hline
Total & 0.01 & 0.99
\end{tabular}
$$
\break
\break
\break
$$
$$P(T)=P(T\cap D)+P(T\cap D')$$
$$P(T|D)=0.99$$
$$P(T'|D')=0.995$$
$$P(T\cap D)=P(D)P(T|D)=0.01*0.99=0.0099$$
$$P(T'\cap D')=P(D')P(T'|D')=0.99*0.995=0.98505$$
$$P(D')=P(T'\cap D')+P(T\cap D')=1-0.01=0.99$$
$$P(T\cap D')=P(D')-P(T'\cap D')=0.99-0.98505=0.00495$$
$$P(T)=P(T\cap D)+P(T\cap D')=0.0099+0.00495=0.01485$$
\begin{tabular}{ llll } 
\hline
 & Uses Drugs (D) & Doesn't Use Drugs (D') & Total \\ 
\hline
Positive Test Results (T) & 0.0099 & 0.00495 &0.01485 \\ 
\hline
Negative Test Results (T') & 0.0001 & 0.98505 &0.98515 \\ 
\hline
\hline
Total & 0.01 & 0.99 & 1
\end{tabular}
$$P(D|T)=\frac{P(D\cap T}{P(T)}=\frac{0.0099}{0.1485}=0.0667$$

\end{problem}

\end{document}